examples/echo/Echo01proof.v
@@ -1,4 +1,4 @@
-Require Import Echo0 Echo1 HoareDef SimModSemdouble.
+Require Import Echo0 Echo1 HoareDef SimModSem.
 Require Import Stack3A.
 Require Import Coqlib.
 Require Import ImpPrelude.
@@ -16,7 +16,7 @@ From ExtLib Require Import
      Core.RelDec
      Structures.Maps
      Data.Map.FMapAList.
-Require Import HTacticsdouble ProofMode IPM.
+Require Import HTactics ProofMode IPM.
 Require Import OpenDef STB.
 
 Set Implicit Arguments.
