examples/knot/KnotImp0proof.v
@@ -1,4 +1,4 @@
-Require Import HoareDef SimModSemdouble.
+Require Import HoareDef SimModSem.
 Require Import Coqlib.
 Require Import ImpPrelude.
 Require Import Skeleton.
@@ -15,13 +15,13 @@ From ExtLib Require Import
      Core.RelDec
      Structures.Maps
      Data.Map.FMapAList.
-Require Import HTacticsdouble ProofMode IPM.
+Require Import HTactics ProofMode IPM.
 Require Import OpenDef.
 Require Import Mem1 MemOpen STB.
 
 Require Import Imp.
 Require Import ImpNotations.
-Require Import ImpProofs2.
+Require Import ImpProofs.
 
 Require Import Knot0 KnotImp.
 
