examples/knot/KnotMain01proof.v
@@ -1,4 +1,4 @@
-Require Import HoareDef KnotHeader KnotMain0 KnotMain1 Knot1 SimModSemdouble.
+Require Import HoareDef KnotHeader KnotMain0 KnotMain1 Knot1 SimModSem.
 Require Import Coqlib.
 Require Import ImpPrelude.
 Require Import Skeleton.
@@ -16,7 +16,7 @@ From ExtLib Require Import
      Structures.Maps
      Data.Map.FMapAList.
 
-Require Import HTacticsdouble ProofMode Invariant.
+Require Import HTactics ProofMode Invariant.
 Require Import STB.
 
 Local Open Scope nat_scope.
