examples/repeat/Repeat01proof.v
@@ -1,4 +1,4 @@
-Require Import HoareDef OpenDef STB Repeat0 Repeat1 SimModSemdouble.
+Require Import HoareDef OpenDef STB Repeat0 Repeat1 SimModSem.
 Require Import Coqlib.
 Require Import ImpPrelude.
 Require Import Skeleton.
@@ -16,11 +16,11 @@ From ExtLib Require Import
      Structures.Maps
      Data.Map.FMapAList.
 
-Require Import HTacticsdouble ProofMode Invariant.
+Require Import HTactics ProofMode Invariant.
 
 Require Import Imp.
 Require Import ImpNotations.
-Require Import ImpProofs2.
+Require Import ImpProofs.
 
 Set Implicit Arguments.
 
