spc/Hoareproof2.v
@@ -8,8 +8,8 @@ Require Import PCM.
 Require Import Any.
 Require Import SimSTS.
 Require Import HoareDef.
-Require Import SimModSemdouble.
-Require Import HTacticsdouble.
+Require Import SimModSem.
+Require Import HTactics.
 From Ordinal Require Import Ordinal Arithmetic.
 
 Set Implicit Arguments.
